Cslib/Computability/Machines/MultiTapeTuring/EqualRoutine.lean
@@ -1,0 +1,39 @@
+/-
+Copyright (c) 2026 Christian Reitwiessner. All rights reserved.
+Released under Apache 2.0 license as described in the file LICENSE.
+Authors: Christian Reitwiessner
+-/
+
+module
+
+import Cslib.Foundations.Data.BiTape
+import Cslib.Foundations.Data.RelatesInSteps
+
+public import Cslib.Computability.Machines.MultiTapeTuring.Basic
+public import Cslib.Computability.Machines.MultiTapeTuring.ListEncoding
+public import Cslib.Computability.Machines.MultiTapeTuring.HeadStats
+
+namespace Turing
+
+namespace Routines
+
+--- A 3-tape Turing machine that pushes the new word "1"
+--- to the third tape if the first words on the first and second tape are the same
+--- and otherwise pushes the empty word to the third tape.
+public def eq : MultiTapeTM 3 (WithSep OneTwo) where
+  Λ := PUnit
+  q₀ := 0
+  M _ syms := sorry
+
+@[simp]
+public theorem eq_eval_list (w₁ w₂ : List OneTwo) (ws₁ ws₂ ws₃ : List (List OneTwo)) :
+  eq.eval_list [w₁ :: ws₁, w₂ :: ws₂, ws₃].get =
+    Part.some (if w₁ = w₂ then
+      [w₁ :: ws₁, w₂ :: ws₂, [.one] :: ws₃].get
+    else
+      [w₁ :: ws₁, w₂ :: ws₂, [] :: ws₃].get) := by
+  sorry
+
+end Routines
+
+end Turing
