Cslib/Computability/Machines/MultiTapeTuring/GraphReachability.lean
@@ -1,0 +1,101 @@
+/-
+Copyright (c) 2026 Christian Reitwiessner. All rights reserved.
+Released under Apache 2.0 license as described in the file LICENSE.
+Authors: Christian Reitwiessner
+-/
+
+module
+
+import Cslib.Foundations.Data.BiTape
+import Cslib.Foundations.Data.RelatesInSteps
+
+public import Cslib.Computability.Machines.MultiTapeTuring.Basic
+public import Cslib.Computability.Machines.MultiTapeTuring.ListEncoding
+public import Cslib.Computability.Machines.MultiTapeTuring.HeadStats
+
+-- TODO create a "common file"
+import Cslib.Computability.Machines.SingleTapeTuring.Basic
+
+namespace Turing
+
+
+-- This is an attempt at proving Savitch's theorem. We start by stating a generic
+-- space-efficient graph reachability algorithm.
+
+/-
+
+General idea, assume distance is power of two:
+
+def reachable(a, b, t, r):
+  if t = 0:
+    return r(a, b)
+  else:
+    for c in vertices:
+      if reachable(a, c, t - 1, r) and reachable(c, b, t - 1, r):
+        return True
+    return False
+
+Until we have a generic mechanism for recursion, let's translate this into a program that
+uses "goto", and every variable is a stack:
+
+def reachable(a, b, t, r):
+  terminate = 0
+  result = 0
+  section = [0]
+  while !terminate:
+    match section.pop()
+    | 0 =>
+      if t = 0:
+        result = r(a, b)
+        terminate = 1
+        section.push(7)
+      else:
+        section.push(1)
+    | 1 =>
+      c.push(0)
+      section.push(2)
+    | 2 =>
+      if c.top() = num_vertices:
+        section.push(6)
+      else:
+        a.push(a.top())
+        b.push(c.top())
+        section.push(0)
+        t.push(t.top() - 1)
+        section.push(3)
+    | 3 =>
+      section.push(4)
+
+
+
+-/
+
+
+
+namespace Routines
+
+variable [Inhabited α] [Fintype α]
+
+public def copy : MultiTapeTM 2 (WithSep α) where
+  Λ := PUnit
+  q₀ := 0
+  M _ syms := sorry
+
+@[simp]
+public lemma copy_eval_list {w : List α} {ls₁ ls₂ : List (List α)} :
+  copy.eval_list [w :: ls₁, ls₂].get = Part.some [w :: ls₁, w :: ls₂].get := by
+  sorry
+
+public lemma copy_evalWithStats {w : List α} {ls₁ ls₂ : List (List α)} :
+  copy.evalWithStats_list #v[w :: ls₁, ls₂].get =
+    .some (
+      [w :: ls₁, w :: ls₂].get,
+      [⟨-1, w.length, 0, by omega⟩, ⟨-w.length - 2, 0, -w.length - 1, by omega⟩].get) := by
+  sorry
+
+-- TODO at some point, we might not want exact stats but rather an upper bound.
+-- Can this be made compatible with using equality?
+
+end Routines
+
+end Turing
