Cslib/Computability/Machines/MultiTapeTuring/IteCombinator.lean
@@ -1,0 +1,42 @@
+/-
+Copyright (c) 2026 Christian Reitwiessner. All rights reserved.
+Released under Apache 2.0 license as described in the file LICENSE.
+Authors: Christian Reitwiessner
+-/
+
+module
+
+import Cslib.Foundations.Data.BiTape
+import Cslib.Foundations.Data.RelatesInSteps
+
+public import Cslib.Computability.Machines.MultiTapeTuring.Basic
+public import Cslib.Computability.Machines.MultiTapeTuring.ListEncoding
+public import Cslib.Computability.Machines.MultiTapeTuring.HeadStats
+
+namespace Turing
+
+namespace Routines
+
+variable [Inhabited α] [Fintype α]
+variable {k : ℕ}
+
+--- Repeatedly run a sub routine as long as a condition on the symbol
+--- at the first head is true.
+public def ite (tm₁ tm₂ : MultiTapeTM k.succ (WithSep α)) :
+    MultiTapeTM k.succ (WithSep α) where
+  Λ := PUnit
+  q₀ := 0
+  M _ syms := sorry
+
+@[simp]
+public theorem ite_eval
+  (tm₁ tm₂ : MultiTapeTM k.succ (WithSep α))
+  (tapes : Fin k.succ → List (List α))
+  (h_nonempty : tapes 0 ≠ []) :
+  (ite tm₁ tm₂).eval_list tapes =
+    if (tapes 0).head h_nonempty = [] then tm₂.eval_list tapes else tm₁.eval_list tapes := by
+  sorry
+
+end Routines
+
+end Turing
