Cslib/Computability/Machines/MultiTapeTuring/SequentialCombinator.lean
@@ -1,0 +1,45 @@
+/-
+Copyright (c) 2026 Christian Reitwiessner. All rights reserved.
+Released under Apache 2.0 license as described in the file LICENSE.
+Authors: Christian Reitwiessner
+-/
+
+module
+
+import Cslib.Foundations.Data.BiTape
+import Cslib.Foundations.Data.RelatesInSteps
+
+public import Cslib.Computability.Machines.MultiTapeTuring.Basic
+public import Cslib.Computability.Machines.MultiTapeTuring.ListEncoding
+public import Cslib.Computability.Machines.MultiTapeTuring.HeadStats
+
+namespace Turing
+
+namespace Routines
+
+variable [Inhabited α] [Fintype α]
+variable {k : ℕ}
+
+--- Run tm₂ after tm₁ has terminated.
+public def seq (tm₁ tm₂ : MultiTapeTM k α) : MultiTapeTM k α := sorry
+
+
+public theorem seq_eval
+  (tm₁ tm₂ : MultiTapeTM k α)
+  (tapes₀ : Fin k → BiTape α) :
+  (seq tm₁ tm₂).eval tapes₀ =
+    tm₁.eval tapes₀ >>= fun tape₁ => tm₂.eval tape₁ := by
+  sorry
+
+public theorem seq_eval_list
+  (tm₁ tm₂ : MultiTapeTM k (WithSep α))
+  (tapes₀ : Fin k → List (List α)) :
+  (seq tm₁ tm₂).eval_list tapes₀ =
+    tm₁.eval_list tapes₀ >>= fun tape₁ => tm₂.eval_list tape₁ := by
+  sorry
+
+
+
+end Routines
+
+end Turing
