Cslib/Computability/Machines/MultiTapeTuring/WhileCombinator.lean
@@ -1,0 +1,60 @@
+/-
+Copyright (c) 2026 Christian Reitwiessner. All rights reserved.
+Released under Apache 2.0 license as described in the file LICENSE.
+Authors: Christian Reitwiessner
+-/
+
+module
+
+import Cslib.Foundations.Data.BiTape
+import Cslib.Foundations.Data.RelatesInSteps
+
+public import Cslib.Computability.Machines.MultiTapeTuring.Basic
+public import Cslib.Computability.Machines.MultiTapeTuring.ListEncoding
+public import Cslib.Computability.Machines.MultiTapeTuring.HeadStats
+
+namespace Turing
+
+namespace Routines
+
+variable [Inhabited α] [Fintype α]
+variable {k : ℕ}
+
+--- Repeatedly run a sub routine as long as a condition on the symbol
+--- at the first head is true.
+public def doWhileSymbol (cond : Option α → Bool) (tm : MultiTapeTM k.succ α) :
+    MultiTapeTM k.succ α where
+  Λ := PUnit
+  q₀ := 0
+  M _ syms := sorry
+
+@[simp]
+public theorem doWhileSymbol_eval
+  (tm : MultiTapeTM k.succ α)
+  (cond : Option α → Bool)
+  (tapes_seq : ℕ → Fin k.succ → BiTape α)
+  (h_transform : ∀ i, tm.eval (tapes_seq i) = .some (tapes_seq i.succ))
+  (h_stops : ∃ m, ¬cond (tapes_seq m 0).head) :
+  (doWhileSymbol cond tm).eval (tapes_seq 0) = .some (tapes_seq (Nat.find h_stops)) := by
+  sorry
+
+--- Repeatedly run a sub routine as long as the first word on the first tape is non-empty.
+public def doWhile (tm : MultiTapeTM k.succ (WithSep α)) :
+    MultiTapeTM k.succ (WithSep α) where
+  Λ := PUnit
+  q₀ := 0
+  M _ syms := sorry
+
+@[simp]
+public theorem doWhile_eval
+  (tm : MultiTapeTM k.succ (WithSep α))
+  (tapes_seq : ℕ → Fin k.succ → List (List α))
+  (h_transform : ∀ i, tm.eval_list (tapes_seq i) = .some (tapes_seq i.succ))
+  (h_nonempty : ∀ i, tapes_seq i 0 ≠ [])
+  (h_stops : ∃ m, (tapes_seq m 0).head (h_nonempty m) = []) :
+  (doWhile tm).eval_list (tapes_seq 0) = .some (tapes_seq (Nat.find h_stops)) := by
+  sorry
+
+end Routines
+
+end Turing
